src/Lustre/Normalization/LNormalization.v
@@ -1,7 +1,7 @@
 From Velus Require Import Common Ident.
 From Velus Require Import Operators Environment.
 From Velus Require Import CoindStreams.
-From Velus Require Import Lustre.LSyntax Lustre.LOrdered Lustre.LTyping Lustre.LSemantics.
+From Velus Require Import Lustre.LSyntax Lustre.LOrdered Lustre.LTyping Lustre.LClocking Lustre.LSemantics.
 From Velus Require Import Lustre.Normalization.Normalization Lustre.Normalization.Correctness Lustre.Normalization.Completeness.
 
 Local Set Warnings "-masking-absolute-name".
@@ -12,10 +12,11 @@ Module Type LNORMALIZATION
        (Import Str : COINDSTREAMS Op OpAux)
        (Import Syn : LSYNTAX Ids Op)
        (Import Typ : LTYPING Ids Op Syn)
+       (Import Clo : LCLOCKING Ids Op Syn)
        (Import Lord : LORDERED Ids Op Syn)
        (Import Sem : LSEMANTICS Ids Op OpAux Syn Lord Str).
-  Declare Module Export Norm : NORMALIZATION Ids Op OpAux Syn Typ.
-  Declare Module Export Correct : CORRECTNESS Ids Op OpAux Str Syn Typ Lord Sem Norm.
+  Declare Module Export Norm : NORMALIZATION Ids Op OpAux Syn.
+  Declare Module Export Correct : CORRECTNESS Ids Op OpAux Str Syn Typ Clo Lord Sem Norm.
   Declare Module Export Complete : COMPLETENESS Ids Op OpAux Syn Typ Norm.
 End LNORMALIZATION.
 
@@ -26,10 +27,11 @@ Module LNormalizationFun
        (Str : COINDSTREAMS Op OpAux)
        (Syn : LSYNTAX Ids Op)
        (Typ : LTYPING Ids Op Syn)
+       (Clo : LCLOCKING Ids Op Syn)
        (Lord : LORDERED Ids Op Syn)
        (Sem : LSEMANTICS Ids Op OpAux Syn Lord Str)
-       <: LNORMALIZATION Ids Op OpAux Str Syn Typ Lord Sem.
-  Module Export Norm := NormalizationFun Ids Op OpAux Syn Typ.
-  Module Export Correct := CorrectnessFun Ids Op OpAux Str Syn Typ Lord Sem Norm.
+       <: LNORMALIZATION Ids Op OpAux Str Syn Typ Clo Lord Sem.
+  Module Export Norm := NormalizationFun Ids Op OpAux Syn.
+  Module Export Correct := CorrectnessFun Ids Op OpAux Str Syn Typ Clo Lord Sem Norm.
   Module Export Complete := CompletenessFun Ids Op OpAux Syn Typ Norm.
 End LNormalizationFun.
